Prove lifting with bracket abstraction
In dire need of a thorough clean-up.

src/Idiomatic_Terms.thy
@@ -3,7 +3,7 @@
 subsection \<open>Idiomatic terms -- Properties and operations\<close>
 
 theory Idiomatic_Terms
-imports Beta_Eta "~~/src/HOL/Library/Permutation"
+imports Beta_Eta
 begin
 
 text \<open>
@@ -322,23 +322,6 @@ proof -
   ultimately show ?thesis by (auto intro: wrap_abs_equiv)
 qed
 
-lemma unlift_all_pure: "opaque x = [] \<Longrightarrow> x \<simeq> Pure (unlift x)"
-proof (induction x)
-  case (Opaque x) then show ?case by simp
-next
-  case (Pure x) then show ?case by simp
-next
-  case (IAp x y)
-  then have no_opaque: "opaque x = []" "opaque y = []" by simp+
-  then have unlift_ap: "unlift (x \<diamondop> y) = unlift x \<degree> unlift y"
-    unfolding unlift_ap by simp
-  from no_opaque IAp.IH have "x \<diamondop> y \<simeq> Pure (unlift x) \<diamondop> Pure (unlift y)"
-    by (blast intro: ap_cong)
-  also have "... \<simeq> Pure (unlift x \<degree> unlift y)" by (rule itrm_hom')
-  also have "... = Pure (unlift (x \<diamondop> y))" by (simp only: unlift_ap)
-  finally show ?case .
-qed
-
 
 subsubsection \<open>Canonical forms\<close>
 
@@ -574,7 +557,7 @@ qed
 
 subsubsection \<open>Lifting with bracket abstraction\<close>
 
-text \<open>Idioms which satisfy additional equations\<close>
+paragraph \<open>Idioms which satisfy additional equations\<close>
 
 locale itrm_ext =
   fixes E :: "'a itrm \<Rightarrow> 'a itrm \<Rightarrow> bool"
@@ -598,7 +581,7 @@ by (induction pred: itrm_cong) (auto intro: itrm_cong.intros idiom_ext[THEN pred
 end
 
 
-text \<open>General notion of bracket abstraction for lambda terms\<close>
+paragraph \<open>General notion of bracket abstraction for lambda terms\<close>
 
 definition foldr_option :: "('a \<Rightarrow> 'b \<Rightarrow> 'b option) \<Rightarrow> 'a list \<Rightarrow> 'b \<Rightarrow> 'b option"
 where "foldr_option f xs e = foldr (\<lambda>a b. Option.bind b (f a)) xs (Some e)"
@@ -620,26 +603,357 @@ definition frees :: "dB \<Rightarrow> nat set"
 where [simp]: "frees t = {i. free t i}"
 
 definition term_dist :: "nat list \<Rightarrow> dB \<Rightarrow> dB"
-where [simp]: "term_dist = fold (\<lambda>i t. t \<degree> Var i)"
+where "term_dist = fold (\<lambda>i t. t \<degree> Var i)"
 
-definition strip_context :: "nat \<Rightarrow> dB \<Rightarrow> dB"
-where "strip_context n t = (THE t'. t = liftn n t 0)"
+lemma upt_eq_Cons_Suc: "[i..<j] = k # ks \<Longrightarrow> [Suc i..<j] = ks"
+by (auto iff: upt_eq_Cons_conv)
+
+lemma upt_last: "[i..<j] = xs @ [x] \<Longrightarrow> i < j \<and> x = j - 1 \<and> xs = [i..<j-1]"
+by (cases j) (auto split: if_splits)
+
+lemma rev_upt_Cons: "x # xs = rev [i..<j] \<Longrightarrow> i < j \<and> x = j - 1 \<and> xs = rev [i..<j-1]"
+by (auto dest!: rev_eq_Cons_iff[THEN iffD1, OF sym] upt_last simp add: rev_swap)
+
+lemma liftn_lift_swap: "liftn n (lift t k) k = lift (liftn n t k) k"
+by (induction n) simp_all
+
+lemma term_dist_Nil[simp]: "term_dist [] t = t"
+unfolding term_dist_def by simp
+
+lemma term_dist_Cons[simp]: "term_dist (v # vs) t = term_dist vs (t \<degree> Var v)"
+unfolding term_dist_def by simp
+
+lemma term_dist_append: "term_dist (vs @ [v]) t = term_dist vs t \<degree> Var v"
+unfolding term_dist_def by simp
+
+lemma term_dist_frees: "frees (term_dist vs t) = frees t \<union> set vs"
+by (induction vs arbitrary: t) auto
+
+lemma term_dist_subst_lt: "\<forall>v\<in>set vs. i < v \<Longrightarrow> (term_dist vs s)[t/i] = term_dist (map (\<lambda>v. v - 1) vs) (s[t/i])"
+by (induction vs arbitrary: s) simp_all
+
+lemma term_dist_subst_gt: "\<forall>v\<in>set vs. v < i \<Longrightarrow> (term_dist vs s)[t/i] = term_dist vs (s[t/i])"
+by (induction vs arbitrary: s) simp_all
+
+definition vsubst :: "nat \<Rightarrow> nat \<Rightarrow> nat \<Rightarrow> nat"
+where "vsubst u v w = (if u < w then u else if u = w then v else u - 1)"
+
+lemma vsubst_subst[simp]: "(Var u)[Var v/w] = Var (vsubst u v w)"
+unfolding vsubst_def by simp
+
+lemma vsubst_subst_lt[simp]: "u < w \<Longrightarrow> vsubst u v w = u"
+unfolding vsubst_def by simp
+
+lemma term_dist_subst_Var: "(term_dist vs s)[Var i/j] = term_dist (map (\<lambda>v. vsubst v i j) vs) (s[Var i/j])"
+by (induction vs arbitrary: s) simp_all
+
+lemma term_dist_cong: "s \<leftrightarrow> t \<Longrightarrow> term_dist vs s \<leftrightarrow> term_dist vs t"
+by (induction vs arbitrary: s t) (auto intro: equiv_appL)
+
+lemma wrap_abs_subst: "(wrap_abs s n)[t/k] = wrap_abs (s[liftn n t 0/k+n]) n"
+by (induction n arbitrary: t k) (simp_all add: liftn_lift_swap)
+
+lemma wrap_abs_beta: "wrap_abs s (Suc n) \<degree> t \<leftrightarrow> wrap_abs (s[liftn n t 0/n]) n"
+proof -
+  have "wrap_abs s (Suc n) \<degree> t = Abs (wrap_abs s n) \<degree> t" by simp
+  also have "... \<leftrightarrow> (wrap_abs s n)[t/0]" by (rule red_into_equiv) blast
+  also have "... = wrap_abs (s[liftn n t 0/n]) n" by (simp add: wrap_abs_subst)
+  finally show ?thesis .
+qed
+
+lemma wrap_abs_dist_eta: "wrap_abs (term_dist (rev [0..<n]) (liftn n t 0)) n \<leftrightarrow> t"
+proof (induction n)
+  case 0 show ?case by simp
+next
+  case (Suc n)
+  let ?dist_range = "\<lambda>a k. term_dist (rev [a..<k]) (liftn k t 0)"
+  have append: "rev [0..<Suc n] = rev [1..<Suc n] @ [0]" by (simp add: upt_rec)
+  have dist_last: "?dist_range 0 (Suc n) = ?dist_range 1 (Suc n) \<degree> Var 0"
+    unfolding append term_dist_append ..
+  have "\<not> free (?dist_range 1 (Suc n)) 0" proof -
+    have "frees (?dist_range 1 (Suc n)) = frees (liftn (Suc n) t 0) \<union> {1..n}"
+      unfolding term_dist_frees by fastforce
+    then have "0 \<notin> frees (?dist_range 1 (Suc n))" by simp
+    then show ?thesis by simp
+  qed
+  then have "Abs (?dist_range 0 (Suc n)) \<rightarrow>\<^sub>\<eta> (?dist_range 1 (Suc n))[Var 0/0]"
+    unfolding dist_last by (rule eta)
+  also have "... = term_dist (rev [0..<n]) ((liftn (Suc n) t 0)[Var 0/0])" proof -
+    have "\<forall>v\<in>set (rev [1..<Suc n]). 0 < v" by auto
+    moreover have "rev [0..<n] = map (\<lambda>v. v - 1) (rev [1..<Suc n])" by (induction n) simp_all
+    ultimately show ?thesis by (simp only: term_dist_subst_lt)
+  qed
+  also have "... = ?dist_range 0 n" using subst_liftn[of 0 n 0 t "Var 0"] by simp
+  finally have "Abs (?dist_range 0 (Suc n)) \<leftrightarrow> ?dist_range 0 n"
+    by (blast intro!: red_into_equiv[OF r_into_rtranclp])
+  then have "wrap_abs (?dist_range 0 (Suc n)) (Suc n) \<leftrightarrow> wrap_abs (?dist_range 0 n) n"
+    unfolding wrap_abs_inside by (rule wrap_abs_equiv)
+  also from Suc.IH have "... \<leftrightarrow> t" .
+  finally show ?case .
+qed
+
+primrec strip_context :: "nat \<Rightarrow> dB \<Rightarrow> nat \<Rightarrow> dB"
+where
+    "strip_context n (Var i) k = (if i < k then Var i else Var (i - n))"
+  | "strip_context n (Abs t) k = Abs (strip_context n t (Suc k))"
+  | "strip_context n (s \<degree> t) k = strip_context n s k \<degree> strip_context n t k"
+
+lemma strip_context_liftn: "strip_context n (liftn (m + n) t k) k = liftn m t k"
+by (induction t arbitrary: k) simp_all
+
+lemma liftn_strip_context:
+  assumes "\<forall>i\<in>frees t. i < k \<or> k + n \<le> i"
+    shows "liftn n (strip_context n t k) k = t"
+using assms proof (induction t arbitrary: k)
+  case (Abs t)
+  then show ?case
+    apply clarsimp
+    by (metis less_imp_Suc_add linorder_not_le not_less_eq plus_nat.simps(2))
+qed auto
+
+lemma liftn_rel_imp_strip_context:
+  assumes "\<forall>i\<in>frees s. i < k \<or> k + n \<le> i"
+      and "\<And>t. P (liftn n t k) t"
+    shows "P s (strip_context n s k)"
+proof -
+  from assms(1) have "liftn n (strip_context n s k) k = s" by (rule liftn_strip_context)
+  with assms(2)[of "strip_context n s k"] show ?thesis by simp
+qed
+
+lemma wrap_abs_dist_eta_free:
+  assumes "\<forall>i\<in>frees t. n \<le> i"
+  shows "wrap_abs (term_dist (rev [0..<n]) t) n \<leftrightarrow> strip_context n t 0"
+apply (rule liftn_rel_imp_strip_context)
+using assms apply simp
+apply (rule wrap_abs_dist_eta)
+done
+
+lemma on_set_eq_imp_map_eq: "\<forall>x\<in>set xs. P x \<Longrightarrow> (\<And>x. P x \<Longrightarrow> f x = g x) \<Longrightarrow> map f xs = map g xs"
+by auto
 
 lemma dist_perm_eta:
-  assumes vars_perm: "vs <~~> [0..<n]"
+  fixes vs
+  defines "n \<equiv> length vs"
+  assumes vars_perm: "bij_betw (\<lambda>i. vs ! i) {0..<n} {0..<n}"
+  obtains vs' where "\<And>t. \<forall>i\<in>frees t. n \<le> i \<Longrightarrow> wrap_abs (term_dist vs' (wrap_abs (term_dist vs (liftn n t 0)) n)) n \<leftrightarrow> strip_context n t 0"
+proof -
+  let ?app_vars = "\<lambda>t n vs' vs. term_dist vs' (wrap_abs (term_dist vs (liftn n t 0)) n)"
+  let ?appd_vars = "\<lambda>t n. term_dist (rev [0..<n]) t"
+
+  def vsubsts \<equiv> "\<lambda>n vs' vs. map (\<lambda>v. if v < n - length vs' then v else if v < n then vs' ! (n - v - 1) + (n - length vs') else v - length vs') vs"
+
+  {
+    fix t and vs vs' :: "nat list"
+    assume p: "length vs' \<le> n"
+
+    let ?m = "n - length vs'"
+    have "?app_vars t n vs' vs \<leftrightarrow> wrap_abs (term_dist (vsubsts n vs' vs) (liftn ?m t 0)) ?m"
+    using p proof (induction vs' arbitrary: vs n)
+      case Nil
+      then have "vsubsts n [] vs = vs" unfolding vsubsts_def by (auto intro: map_idI)
+      then show ?case by simp
+    next
+      case (Cons v vs')
+      let ?mm = "n - length (v # vs')"
+      let ?mm' = "(n - 1) - length vs'"
+      from Cons.prems have vs'_length: "length vs' \<le> n - 1" by simp
+      from Cons.prems have "0 < n" by simp
+      then have "?app_vars t n (v # vs') vs = ?app_vars t (Suc (n-1)) (v # vs') vs" by simp
+      also have "... \<leftrightarrow> term_dist vs' (wrap_abs ((term_dist vs (liftn (Suc (n-1)) t 0))[liftn (n-1) (Var v) 0/n-1]) (n-1))"
+        apply (unfold term_dist_Cons)
+        apply (rule term_dist_cong)
+        apply (rule wrap_abs_beta)
+        done
+      also have "... = term_dist vs' (wrap_abs (term_dist (vsubsts n [v] vs) (liftn (n-1) t 0)) (n-1))"
+      proof -
+        have 1: "v + n - 1 = v + (n - 1)" using `n > 0` by simp
+        have "(term_dist vs (liftn (Suc (n-1)) t 0))[Var (v + n - 1)/n-1] =
+          term_dist (map (\<lambda>v'. vsubst v' (v + n - 1) (n-1)) vs) ((liftn (Suc (n-1)) t 0)[Var (v + n - 1)/n-1])"
+          using term_dist_subst_Var .
+        also have "... = term_dist (vsubsts n [v] vs) (liftn (n-1) t 0)"
+        proof -
+          have "map (\<lambda>v'. vsubst v' (v + n - 1) (n-1)) vs = vsubsts n [v] vs"
+            unfolding vsubsts_def vsubst_def
+            using `n > 0`
+            by (auto cong: if_cong)
+          then show ?thesis using `n > 0`
+            by (metis One_nat_def Suc_pred le_add1 less_Suc_eq_le subst_liftn)
+        qed
+        finally show ?thesis unfolding 1 by simp
+      qed
+      also have "... \<leftrightarrow> wrap_abs (term_dist (vsubsts (n-1) vs' (vsubsts n [v] vs)) (liftn ?mm' t 0)) ?mm'"
+      using vs'_length Cons.IH by blast
+      also have "... = wrap_abs (term_dist (vsubsts n (v # vs') vs) (liftn ?mm t 0)) ?mm"
+      proof -
+        have 1: "length [v] = 1" by simp
+        have "?mm' = ?mm" by simp
+        moreover have "vsubsts (n-1) vs' (vsubsts n [v] vs) = vsubsts n (v # vs') vs"
+          unfolding vsubsts_def map_map comp_def
+          apply (rule map_cong)
+          apply rule
+          apply (unfold 1)
+          apply (split split_if)+
+          apply safe
+          apply clarsimp
+          apply clarsimp
+          apply clarsimp
+          apply clarsimp
+          apply clarsimp
+          apply clarsimp
+          apply clarsimp
+          apply clarsimp
+          apply clarsimp
+          apply clarsimp
+          apply clarsimp
+          apply clarsimp
+          apply clarsimp
+          apply clarsimp
+          apply clarsimp
+          apply clarsimp
+          using vs'_length
+          apply clarsimp
+          apply clarsimp
+          apply clarsimp
+          apply clarsimp
+          apply clarsimp
+          apply arith
+          apply clarsimp
+          apply clarsimp
+          apply clarsimp
+          apply clarsimp
+          defer
+          apply clarsimp
+          apply clarsimp
+          apply clarsimp
+          apply arith
+          apply clarsimp
+          using vs'_length
+          apply(cases n)
+          apply simp_all
+          done
+        ultimately show ?thesis by simp
+      qed
+      finally show ?case .
+    qed
+  }
+  note 1 = this
+
+  def solution \<equiv> "map (\<lambda>i. n - the_inv_into {0..<n} (\<lambda>j. vs ! j) (n - i - 1) - 1) [0..<n]"
+
+  have all_vs: "\<forall>v\<in>set vs. v < n" proof
+    fix v assume "v \<in> set vs"
+    then obtain i where "i < length vs" and "vs ! i = v"
+      by (blast dest: in_set_conv_nth[THEN iffD1])
+    then have "vs ! i \<in> {0..<n}"
+      using vars_perm unfolding n_def by (auto dest: bij_betwE)
+    then show "v < n" unfolding `vs ! i = v` by simp
+  qed
+
+  have solution_length: "length solution = n" unfolding solution_def by simp
+  have "\<And>v. v < n \<Longrightarrow> solution ! (n - v - 1) = n - the_inv_into {0..<n} (\<lambda>j. vs ! j) v - 1"
+    unfolding n_def solution_def by auto
+  with vars_perm have "map (\<lambda>v. solution ! (n - v - 1)) vs = rev [0..<n]"
+    apply (subst list.rel_eq[symmetric])
+    apply (subst list.rel_map)
+    apply (rule list_all2_all_nthI)
+    apply (unfold n_def)
+    apply clarsimp
+    apply (subgoal_tac "vs ! n < length vs")
+    apply clarsimp
+    apply (auto dest!: bij_betw_imp_inj_on iff: the_inv_into_f_eq rev_nth)[1]
+    apply (auto dest: bij_betwE)
+    done
+  then have solution_vs: "vsubsts n solution vs = rev [0..<n]"
+    unfolding vsubsts_def solution_length
+    using all_vs
+    apply (elim on_set_eq_imp_map_eq [where g="\<lambda>v. solution ! (n - v - 1)", THEN trans])
+    apply simp_all
+    done
+  {
+    fix t
+    assume not_free: "\<forall>i\<in>frees t. n \<le> i"
+    have "?app_vars t n solution vs \<leftrightarrow> ?appd_vars t n" for t
+      using 1[of solution vs t] solution_length solution_vs by auto
+    then have "wrap_abs (?app_vars t n solution vs) n \<leftrightarrow> wrap_abs (?appd_vars t n) n"
+      by (rule wrap_abs_equiv)
+    also have "... \<leftrightarrow> strip_context n t 0"
+      using not_free by (rule wrap_abs_dist_eta_free)
+    finally have "wrap_abs (?app_vars t n solution vs) n \<leftrightarrow> ..." .
+  }
+  with that show ?thesis .
+qed
+
+lemma liftn_wrap_abs: "liftn n (wrap_abs t m) k = wrap_abs (liftn n t (k + m)) m"
+by (induction m arbitrary: k) auto
+
+lemma liftn_term_dist_lt: "\<forall>i\<in>set vs. i < k \<Longrightarrow> liftn n (term_dist vs t) k = term_dist vs (liftn n t k)"
+by (induction vs arbitrary: t) auto
+
+lemma liftn_context_conv: "k \<le> k' \<Longrightarrow> \<forall>i\<in>frees t. i < k \<or> k' \<le> i \<Longrightarrow> liftn n t k = liftn n t k'"
+proof (induction t arbitrary: k k')
+  case (Abs t)
+  have "\<forall>i\<in>frees t. i < Suc k \<or> Suc k' \<le> i" proof
+    fix i assume "i \<in> frees t"
+    show "i < Suc k \<or> Suc k' \<le> i" proof (cases "i = 0")
+      assume "i = 0" then show ?thesis by simp
+    next
+      assume "i \<noteq> 0"
+      from Abs.prems(2) have "\<forall>i. free t (Suc i) \<longrightarrow> i < k \<or> k' \<le> i" by auto
+      with `i \<noteq> 0` `i \<in> frees t` show ?thesis
+        by (metis frees_def less_Suc_eq_0_disj linorder_not_le mem_Collect_eq)
+    qed
+  qed
+  with Abs.IH Abs.prems(1) show ?case by auto
+qed auto
+
+lemma liftn_liftn0: "\<forall>i\<in>frees t. k \<le> i \<Longrightarrow> liftn n t k = liftn n t 0"
+using liftn_context_conv by auto
+
+lemma dist_perm_eta_equiv:
+  fixes vs
+  defines "n \<equiv> length vs"
+  assumes vars_perm: "bij_betw (op ! vs) {0..<n} {0..<n}"
       and not_free: "\<forall>i\<in>frees s. n \<le> i" "\<forall>i\<in>frees t. n \<le> i"
       and perm_equiv: "wrap_abs (term_dist vs s) n \<leftrightarrow> wrap_abs (term_dist vs t) n"
-    shows "strip_context n s \<leftrightarrow> strip_context n t"
-(*
-  TODO:
-  - find permutation vs' such that rev vs' o vs = rev [0..<n]
-  - show "term_dist vs' (wrap_abs (term_dist vs (liftn n s 0)) n) \<leftrightarrow> term_dist (rev [0..<n]) s"
-    by repeated beta-reduction, likewise for t
-  - show "wrap_abs (term_dist (rev [0..<n]) s) n \<leftrightarrow> strip_context n s" by repeated eta-reduction
-    using not_free, likewise for t
-  - compose everything with theorems like liftn_equiv, wrap_abs_equiv, etc.
-*)
-oops
+    shows "strip_context n s 0 \<leftrightarrow> strip_context n t 0"
+proof -
+  have all_vs: "\<forall>v\<in>set vs. v < n" proof
+    fix v assume "v \<in> set vs"
+    then obtain i where "i < length vs" and "vs ! i = v"
+      by (blast dest: in_set_conv_nth[THEN iffD1])
+    then have "vs ! i \<in> {0..<n}"
+      using vars_perm unfolding n_def by (auto dest: bij_betwE)
+    then show "v < n" unfolding `vs ! i = v` by simp
+  qed
+
+  obtain vs' where
+    etas: "\<And>t. \<forall>i\<in>frees t. n \<le> i \<Longrightarrow> wrap_abs (term_dist vs' (wrap_abs (term_dist vs (liftn n t 0)) n)) n \<leftrightarrow> strip_context n t 0"
+    using dist_perm_eta vars_perm unfolding n_def by blast
+
+  have "strip_context n s 0 \<leftrightarrow> wrap_abs (term_dist vs' (wrap_abs (term_dist vs (liftn n s 0)) n)) n"
+    using etas[THEN term_sym] not_free(1) .
+  also have "... \<leftrightarrow> wrap_abs (term_dist vs' (wrap_abs (term_dist vs (liftn n t 0)) n)) n"
+  proof (rule wrap_abs_equiv, rule term_dist_cong)
+    have "wrap_abs (term_dist vs (liftn n s 0)) n = wrap_abs (term_dist vs (liftn n s n)) n"
+      using not_free(1) liftn_liftn0[of s n] by simp
+    also have "... = wrap_abs (liftn n (term_dist vs s) n) n"
+      using all_vs liftn_term_dist_lt by simp
+    also have "... = liftn n (wrap_abs (term_dist vs s) n) 0"
+      using liftn_wrap_abs by simp
+    also have "... \<leftrightarrow> liftn n (wrap_abs (term_dist vs t) n) 0"
+      using perm_equiv by (rule equiv_liftn)
+    also have "... = wrap_abs (liftn n (term_dist vs t) n) n"
+      using liftn_wrap_abs by simp
+    also have "... = wrap_abs (term_dist vs (liftn n t n)) n"
+      using all_vs liftn_term_dist_lt by simp
+    also have "... = wrap_abs (term_dist vs (liftn n t 0)) n"
+      using not_free(2) liftn_liftn0[of t n] by simp
+    finally show "wrap_abs (term_dist vs (liftn n s 0)) n \<leftrightarrow> ..." .
+  qed
+  also have "... \<leftrightarrow> strip_context n t 0"
+    using etas not_free(2) .
+  finally show ?thesis .
+qed
 
 locale bracket_abstraction =
   fixes term_bracket :: "nat \<Rightarrow> dB \<Rightarrow> dB option"
@@ -648,7 +962,21 @@ locale bracket_abstraction =
 begin
 
 definition term_brackets :: "nat list \<Rightarrow> dB \<Rightarrow> dB option"
-where [simp]: "term_brackets = foldr_option term_bracket"
+where "term_brackets = foldr_option term_bracket"
+
+lemma term_brackets_Nil[simp]: "term_brackets [] t = Some t"
+unfolding term_brackets_def by simp
+
+lemma term_brackets_Cons:
+  assumes "term_brackets (v#vs) t = Some t'"
+  obtains s' where "term_brackets vs t = Some s'" and "term_bracket v s' = Some t'"
+using assms unfolding term_brackets_def by (elim foldr_option_Cons)
+
+lemma term_brackets_ConsI:
+  assumes "term_brackets vs t = Some t'"
+      and "term_bracket v t' = Some t''"
+shows "term_brackets (v#vs) t = Some t''"
+using assms unfolding term_brackets_def foldr_option_def by simp
 
 lemma bracket_dist:
   assumes "term_brackets vs t = Some t'"
@@ -662,7 +990,7 @@ proof -
     from Cons.prems obtain u where
         inner: "term_brackets vs t = Some u" and
         step: "term_bracket v u = Some t'"
-      by (auto elim: foldr_option_Cons)
+      by (auto elim: term_brackets_Cons)
     from step have red1: "t' \<degree> Var v \<leftrightarrow> u" by (rule bracket_app)
     show ?case proof rule+
       fix t'' assume "t' \<leftrightarrow> t''"
@@ -679,37 +1007,74 @@ qed
 end
 
 
-text \<open>Bracket abstraction for idiomatic terms\<close>
+paragraph \<open>Bracket abstraction for idiomatic terms\<close>
+
+text \<open>We consider idiomatic terms with explicitly assigned variables.\<close>
+
+primrec unlift_vars :: "nat \<Rightarrow> nat itrm \<Rightarrow> dB"
+where
+    "unlift_vars n (Opaque i) = Var i"
+  | "unlift_vars n (Pure x) = liftn n x 0"
+  | "unlift_vars n (x \<diamondop> y) = unlift_vars n x \<degree> unlift_vars n y"
+
+lemma strip_unlift_vars:
+  assumes "opaque x = []"
+  shows "strip_context n (unlift_vars n x) 0 = unlift_vars 0 x"
+using assms by (induction x) (simp_all add: strip_context_liftn[where m=0, simplified])
+
+lemma unlift_vars_frees: "\<forall>i\<in>frees (unlift_vars n x). i \<in> set (opaque x) \<or> n \<le> i"
+by (induction x) (auto simp add: free_liftn)
+
+lemma unlift_all_pure: "opaque x = [] \<Longrightarrow> x \<simeq> Pure (unlift_vars 0 x)"
+proof (induction x)
+  case (Opaque x) then show ?case by simp
+next
+  case (Pure x) then show ?case by simp
+next
+  case (IAp x y)
+  then have no_opaque: "opaque x = []" "opaque y = []" by simp+
+  then have unlift_ap: "unlift_vars 0 (x \<diamondop> y) = unlift_vars 0 x \<degree> unlift_vars 0 y"
+    unfolding unlift_ap by simp
+  from no_opaque IAp.IH have "x \<diamondop> y \<simeq> Pure (unlift_vars 0 x) \<diamondop> Pure (unlift_vars 0 y)"
+    by (blast intro: ap_cong)
+  also have "... \<simeq> Pure (unlift_vars 0 x \<degree> unlift_vars 0 y)" by (rule itrm_hom')
+  also have "... = Pure (unlift_vars 0 (x \<diamondop> y))" by (simp only: unlift_ap)
+  finally show ?case .
+qed
 
 locale itrm_abstraction = bracket_abstraction + itrm_ext E for E :: "nat itrm \<Rightarrow> _" +
   fixes itrm_bracket :: "nat \<Rightarrow> nat itrm \<Rightarrow> nat itrm option"
   assumes itrm_bracket_ap: "itrm_bracket i x = Some x' \<Longrightarrow> x' \<diamondop> Opaque i \<simeq>\<^sup>+ x"
   assumes itrm_bracket_opaque: "itrm_bracket i x = Some x' \<Longrightarrow> set (opaque x') = set (opaque x) - {i}"
-  (* FIXME *)
   assumes bracket_compat:
-    "set (opaque x) \<subseteq> set vs \<Longrightarrow>
-      rel_option (op \<leftrightarrow>)
-        (term_brackets vs (unlift' (iorder x) x 0))
-        (map_option unlift (foldr_option itrm_bracket vs x))"
+    "set (opaque x) \<subseteq> {0..<n} \<Longrightarrow> i < n \<Longrightarrow>
+      term_bracket i (unlift_vars n x) = map_option (unlift_vars n) (itrm_bracket i x)"
 begin
 
 definition "itrm_brackets = foldr_option itrm_bracket"
+
+lemma itrm_brackets_Nil[simp]: "itrm_brackets [] x = Some x"
+unfolding itrm_brackets_def by simp
 
 lemma itrm_brackets_Cons:
   assumes "itrm_brackets (v#vs) x = Some x'"
   obtains y' where "itrm_brackets vs x = Some y'" and "itrm_bracket v y' = Some x'"
 using assms unfolding itrm_brackets_def by (elim foldr_option_Cons)
 
-definition "itrm_bracket_norm = fold (\<lambda>i y. y \<diamondop> Opaque i)"
+definition "itrm_dist = fold (\<lambda>i y. y \<diamondop> Opaque i)"
 
-lemma bracket_nf: "itrm_brackets vs x = Some x' \<Longrightarrow> itrm_bracket_norm vs x' \<simeq>\<^sup>+ x"
+lemma itrm_dist_cong: "x \<simeq>\<^sup>+ y \<Longrightarrow> itrm_dist vs x \<simeq>\<^sup>+ itrm_dist vs y"
+unfolding itrm_dist_def
+by (induction vs arbitrary: x y) (simp_all add: ap_congL)
+
+lemma bracket_nf: "itrm_brackets vs x = Some x' \<Longrightarrow> itrm_dist vs x' \<simeq>\<^sup>+ x"
 proof -
   assume defined: "itrm_brackets vs x = Some x'"
   {
     def x'' == x'
     assume "x' \<simeq>\<^sup>+ x''"
-    with defined have "itrm_bracket_norm vs x'' \<simeq>\<^sup>+ x"
-      unfolding itrm_bracket_norm_def
+    with defined have "itrm_dist vs x'' \<simeq>\<^sup>+ x"
+      unfolding itrm_dist_def
       proof (induction vs arbitrary: x' x'')
         case Nil then show ?case unfolding itrm_brackets_def by (simp add: itrm_sym)
       next
@@ -727,9 +1092,19 @@ proof -
   then show ?thesis using itrm_refl .
 qed
 
-lemma bracket_nf_cong: "x \<simeq>\<^sup>+ y \<Longrightarrow> itrm_bracket_norm vs x \<simeq>\<^sup>+ itrm_bracket_norm vs y"
-unfolding itrm_bracket_norm_def
+lemma bracket_nf_cong: "x \<simeq>\<^sup>+ y \<Longrightarrow> itrm_dist vs x \<simeq>\<^sup>+ itrm_dist vs y"
+unfolding itrm_dist_def
 by (induction vs arbitrary: x y) (auto intro: ap_congL)
+
+lemma bracket_not_free:
+  assumes "itrm_brackets vs x = Some x'"
+    shows "set (opaque x') = set (opaque x) - set vs"
+using assms proof (induction vs arbitrary: x')
+  case Nil then show ?case unfolding itrm_brackets_def by simp
+next
+  case (Cons v vs) then show ?case
+    by (auto elim: itrm_brackets_Cons dest!: itrm_bracket_opaque)
+qed
 
 lemma bracket_complete:
   assumes complete: "set (opaque x) \<subseteq> set vs"
@@ -737,12 +1112,7 @@ lemma bracket_complete:
     shows "opaque x' = []"
 proof -
   from defined have "set (opaque x') = set (opaque x) - set vs"
-    proof (induction vs arbitrary: x')
-      case Nil then show ?case unfolding itrm_brackets_def by simp
-    next
-      case (Cons v vs) then show ?case
-        by (auto elim: itrm_brackets_Cons dest!: itrm_bracket_opaque)
-    qed
+    by (rule bracket_not_free)
   with complete have "set (opaque x') = {}" by simp
   then show ?thesis by simp
 qed
@@ -750,24 +1120,101 @@ qed
 lemma bracket_complete_unlift:
   assumes complete: "set (opaque x) \<subseteq> set vs"
       and defined: "itrm_brackets vs x = Some x'"
-    shows "x' \<simeq>\<^sup>+ Pure (unlift x')"
+    shows "x' \<simeq>\<^sup>+ Pure (unlift_vars 0 x')"
 proof (rule equiv_into_ext)
   from assms have "opaque x' = []" by (rule bracket_complete)
-  then show "x' \<simeq> Pure (unlift x')" by (rule unlift_all_pure)
+  then show "x' \<simeq> Pure (unlift_vars 0 x')" by (rule unlift_all_pure)
+qed
+
+lemma itrm_to_term_brackets:
+  assumes "set (opaque x) \<subseteq> {0..<n}"
+      and "set vs \<subseteq> {0..<n}"
+      and "itrm_brackets vs x = Some x'"
+    shows "term_brackets vs (unlift_vars n x) = Some (unlift_vars n x')"
+using assms(2,3) proof (induction vs arbitrary: x')
+  case Nil then show ?case by simp
+next
+  case (Cons v vs)
+  then obtain y' where ivs: "itrm_brackets vs x = Some y'" and iv: "itrm_bracket v y' = Some x'"
+    by (elim itrm_brackets_Cons)
+  with Cons have "term_brackets vs (unlift_vars n x) = Some (unlift_vars n y')"
+    by auto
+  moreover {
+    have "Some (unlift_vars n x') = map_option (unlift_vars n) (itrm_bracket v y')"
+      unfolding iv by simp
+    moreover have "set (opaque y') \<subseteq> {0..<n}"
+      using assms(1) ivs by (auto dest: bracket_not_free)
+    moreover have "v < n" using Cons.prems by simp
+    ultimately have "term_bracket v (unlift_vars n y') = Some (unlift_vars n x')"
+      using bracket_compat by auto
+  }
+  ultimately show ?case by (rule term_brackets_ConsI)
 qed
 
 theorem bracket_lifting:
-  assumes complete: "set (opaque x) \<subseteq> set vs" "set (opaque y) \<subseteq> set vs" (*FIXME*)
+  fixes vs
+  defines "n \<equiv> length vs"
+  assumes all_vars: "set (opaque x) \<union> set (opaque y) \<subseteq> {0..<n}"
+      and perm_vars: "bij_betw (op ! vs) {0..<n} {0..<n}"
       and defined: "itrm_brackets vs x = Some x'" "itrm_brackets vs y = Some y'"
-      and base_eq: "unlift x \<leftrightarrow> unlift y"
+      and base_eq: "wrap_abs (unlift_vars n x) n \<leftrightarrow> wrap_abs (unlift_vars n y) n"
     shows "x \<simeq>\<^sup>+ y"
 proof -
-  have "x \<simeq>\<^sup>+ itrm_bracket_norm vs x'" using defined(1) by (rule bracket_nf[symmetric])
-  also have "... \<simeq>\<^sup>+ itrm_bracket_norm vs (Pure (unlift x'))"
-    using complete(1) defined(1)
-    by (blast intro: bracket_nf_cong bracket_complete_unlift)
-  (*TODO*)
-oops
+  have set_vs: "set vs = {0..<n}"
+  proof safe+
+    fix v assume "v \<in> set vs"
+    then obtain i where "i < length vs \<and> vs ! i = v" by (auto iff: in_set_conv_nth)
+    then show "v \<in> {0..<n}" using perm_vars[THEN bij_betwE] unfolding n_def by auto
+  next
+    fix v assume "v \<in> {0..<n}"
+    then obtain i where "i < length vs \<and> vs ! i = v"
+      using perm_vars unfolding n_def
+      by (metis (mono_tags) atLeastLessThan_iff bij_betw_imageE imageE)
+    then show "v \<in> set vs" by auto
+  qed
+
+  have compat_x: "term_brackets vs (unlift_vars n x) = Some (unlift_vars n x')"
+    using all_vars set_vs defined(1) by (auto intro: itrm_to_term_brackets)
+  have compat_y: "term_brackets vs (unlift_vars n y) = Some (unlift_vars n y')"
+    using all_vars set_vs defined(2) by (auto intro: itrm_to_term_brackets)
+
+  from all_vars have "set (opaque x) \<subseteq> set vs" unfolding set_vs by simp
+  then have complete_x: "opaque x' = []" using defined(1) bracket_complete by blast
+  then have ux_frees: "\<forall>i\<in>frees (unlift_vars n x'). n \<le> i"
+    using unlift_vars_frees by fastforce
+
+  from all_vars have "set (opaque y) \<subseteq> set vs" unfolding set_vs by simp
+  then have complete_y: "opaque y' = []" using defined(2) bracket_complete by blast
+  then have uy_frees: "\<forall>i\<in>frees (unlift_vars n y'). n \<le> i"
+    using unlift_vars_frees by fastforce
+
+  have "x \<simeq>\<^sup>+ itrm_dist vs x'" using defined(1) by (rule bracket_nf[symmetric])
+  also have "... \<simeq>\<^sup>+ itrm_dist vs (Pure (unlift_vars 0 x'))"
+    using all_vars set_vs defined(1)
+    by (auto intro: bracket_nf_cong bracket_complete_unlift)
+  also have "... \<simeq>\<^sup>+ itrm_dist vs (Pure (unlift_vars 0 y'))"
+  proof (rule itrm_dist_cong, rule pure_subst)
+    have "wrap_abs (term_dist vs (unlift_vars n x')) n \<leftrightarrow> wrap_abs (unlift_vars n x) n"
+      using compat_x bracket_dist by (auto intro: wrap_abs_equiv)
+    also have "... \<leftrightarrow> wrap_abs (unlift_vars n y) n" using base_eq .
+    also have "... \<leftrightarrow> wrap_abs (term_dist vs (unlift_vars n y')) n"
+      using compat_y bracket_dist[THEN term_sym] by (auto intro: wrap_abs_equiv)
+    finally have "strip_context n (unlift_vars n x') 0 \<leftrightarrow> strip_context n (unlift_vars n y') 0"
+      using perm_vars ux_frees uy_frees
+      unfolding n_def
+      by (intro dist_perm_eta_equiv)
+    then show "unlift_vars 0 x' \<leftrightarrow> unlift_vars 0 y'"
+      using strip_unlift_vars complete_x complete_y by simp
+  qed
+  also have "... \<simeq>\<^sup>+ itrm_dist vs y'"
+    using all_vars set_vs defined(2)
+    apply (intro itrm_dist_cong)
+    apply (intro bracket_complete_unlift[THEN itrm_sym])
+    apply auto
+    done
+  also have "... \<simeq>\<^sup>+ y" using defined(2) by (rule bracket_nf)
+  finally show ?thesis .
+qed
 
 end
 
